Change x64 reg type from datatype to integer type

vale/code/arch/x64/X64.Vale.Regs.fst
@@ -2,27 +2,27 @@ module X64.Vale.Regs
 open X64.Machine_s
 
 let of_fun m =
-  let m0_3 = ((m Rax, m Rbx), (m Rcx, m Rdx)) in
-  let m4_7 = ((m Rsi, m Rdi), (m Rbp, m Rsp)) in
-  let m8_11 = ((m R8, m R9), (m R10, m R11)) in
-  let m12_15 = ((m R12, m R13), (m R14, m R15)) in
+  let m0_3 = ((m rRax, m rRbx), (m rRcx, m rRdx)) in
+  let m4_7 = ((m rRsi, m rRdi), (m rRbp, m rRsp)) in
+  let m8_11 = ((m rR8, m rR9), (m rR10, m rR11)) in
+  let m12_15 = ((m rR12, m rR13), (m rR14, m rR15)) in
   let m' = ((m0_3, m4_7), (m8_11, m12_15)) in
-  assert_norm (m Rax == sel Rax m');
-  assert_norm (m Rbx == sel Rbx m');
-  assert_norm (m Rcx == sel Rcx m');
-  assert_norm (m Rdx == sel Rdx m');
-  assert_norm (m Rsi == sel Rsi m');
-  assert_norm (m Rdi == sel Rdi m');
-  assert_norm (m Rbp == sel Rbp m');
-  assert_norm (m Rsp == sel Rsp m');
-  assert_norm (m R8  == sel R8  m');
-  assert_norm (m R9  == sel R9  m');
-  assert_norm (m R10 == sel R10 m');
-  assert_norm (m R11 == sel R11 m');
-  assert_norm (m R12 == sel R12 m');
-  assert_norm (m R13 == sel R13 m');
-  assert_norm (m R14 == sel R14 m');
-  assert_norm (m R15 == sel R15 m');
+  assert_norm (m rRax == sel rRax m');
+  assert_norm (m rRbx == sel rRbx m');
+  assert_norm (m rRcx == sel rRcx m');
+  assert_norm (m rRdx == sel rRdx m');
+  assert_norm (m rRsi == sel rRsi m');
+  assert_norm (m rRdi == sel rRdi m');
+  assert_norm (m rRbp == sel rRbp m');
+  assert_norm (m rRsp == sel rRsp m');
+  assert_norm (m rR8  == sel rR8  m');
+  assert_norm (m rR9  == sel rR9  m');
+  assert_norm (m rR10 == sel rR10 m');
+  assert_norm (m rR11 == sel rR11 m');
+  assert_norm (m rR12 == sel rR12 m');
+  assert_norm (m rR13 == sel rR13 m');
+  assert_norm (m rR14 == sel rR14 m');
+  assert_norm (m rR15 == sel rR15 m');
   m'
 
 let lemma_upd_eq r v m =
@@ -34,8 +34,8 @@ let lemma_upd_ne r r' v m =
 let equal m1 m2 = m1 == m2
 
 let lemma_equal_intro m1 m2 =
-  assert_norm (forall (r:reg). sel r m1 == Map16.sel m1 (reg_to_int r));
-  assert_norm (forall (r:reg). sel r m2 == Map16.sel m2 (reg_to_int r));
+  assert_norm (forall (r:reg). sel r m1 == Map16.sel m1 r);
+  assert_norm (forall (r:reg). sel r m2 == Map16.sel m2 r);
   Map16.lemma_equal m1 m2
 
 let lemma_equal_elim m1 m2 = ()
@@ -43,20 +43,20 @@ let lemma_equal_elim m1 m2 = ()
 let lemma_eta m =
   let m1 = m in
   let m2 = eta m in
-  assert_norm (sel Rax m1 == sel Rax m2);
-  assert_norm (sel Rbx m1 == sel Rbx m2);
-  assert_norm (sel Rcx m1 == sel Rcx m2);
-  assert_norm (sel Rdx m1 == sel Rdx m2);
-  assert_norm (sel Rsi m1 == sel Rsi m2);
-  assert_norm (sel Rdi m1 == sel Rdi m2);
-  assert_norm (sel Rbp m1 == sel Rbp m2);
-  assert_norm (sel Rsp m1 == sel Rsp m2);
-  assert_norm (sel R8  m1 == sel R8  m2);
-  assert_norm (sel R9  m1 == sel R9  m2);
-  assert_norm (sel R10 m1 == sel R10 m2);
-  assert_norm (sel R11 m1 == sel R11 m2);
-  assert_norm (sel R12 m1 == sel R12 m2);
-  assert_norm (sel R13 m1 == sel R13 m2);
-  assert_norm (sel R14 m1 == sel R14 m2);
-  assert_norm (sel R15 m1 == sel R15 m2);
+  assert_norm (sel rRax m1 == sel rRax m2);
+  assert_norm (sel rRbx m1 == sel rRbx m2);
+  assert_norm (sel rRcx m1 == sel rRcx m2);
+  assert_norm (sel rRdx m1 == sel rRdx m2);
+  assert_norm (sel rRsi m1 == sel rRsi m2);
+  assert_norm (sel rRdi m1 == sel rRdi m2);
+  assert_norm (sel rRbp m1 == sel rRbp m2);
+  assert_norm (sel rRsp m1 == sel rRsp m2);
+  assert_norm (sel rR8  m1 == sel rR8  m2);
+  assert_norm (sel rR9  m1 == sel rR9  m2);
+  assert_norm (sel rR10 m1 == sel rR10 m2);
+  assert_norm (sel rR11 m1 == sel rR11 m2);
+  assert_norm (sel rR12 m1 == sel rR12 m2);
+  assert_norm (sel rR13 m1 == sel rR13 m2);
+  assert_norm (sel rR14 m1 == sel rR14 m2);
+  assert_norm (sel rR15 m1 == sel rR15 m2);
   lemma_equal_intro m1 m2
