vale/code/arch/x64/X64.Vale.Regs.fsti
@@ -9,35 +9,13 @@ type regs_def = map16 nat64
 [@"opaque_to_smt"]
 type t = regs_def
 
-type reg_int:eqtype = i:int{0 <= i /\ i < 16}
-
-[@va_qattr]
-let reg_to_int (r:reg) : reg_int =
-  match r with
-  | Rax -> 0
-  | Rbx -> 1
-  | Rcx -> 2
-  | Rdx -> 3
-  | Rsi -> 4
-  | Rdi -> 5
-  | Rbp -> 6
-  | Rsp -> 7
-  | R8 -> 8
-  | R9 -> 9
-  | R10 -> 10
-  | R11 -> 11
-  | R12 -> 12
-  | R13 -> 13
-  | R14 -> 14
-  | R15 -> 15
-
 [@va_qattr "opaque_to_smt"]
 let sel (r:reg) (m:t) : nat64 =
-  sel16 m (reg_to_int r)
+  sel16 m r
 
 [@va_qattr "opaque_to_smt"]
 let upd (r:reg) (v:nat64) (m:t) : t =
-  upd16 m (reg_to_int r) v
+  upd16 m r v
 
 // Used in eta-expansion; we ensure that it stops normalization by not marking it va_qattr
 [@"opaque_to_smt"]
@@ -48,10 +26,10 @@ let eta_sel (r:reg) (m:t) : v:nat64{v == sel r m} =
 // so that we don't accidentally normalize past type abstractions
 [@va_qattr "opaque_to_smt"]
 let eta (m:t) : t =
-  let m0_3 = ((eta_sel Rax m, eta_sel Rbx m), (eta_sel Rcx m, eta_sel Rdx m)) in
-  let m4_7 = ((eta_sel Rsi m, eta_sel Rdi m), (eta_sel Rbp m, eta_sel Rsp m)) in
-  let m8_11 = ((eta_sel R8 m, eta_sel R9 m), (eta_sel R10 m, eta_sel R11 m)) in
-  let m12_15 = ((eta_sel R12 m, eta_sel R13 m), (eta_sel R14 m, eta_sel R15 m)) in
+  let m0_3 = ((eta_sel rRax m, eta_sel rRbx m), (eta_sel rRcx m, eta_sel rRdx m)) in
+  let m4_7 = ((eta_sel rRsi m, eta_sel rRdi m), (eta_sel rRbp m, eta_sel rRsp m)) in
+  let m8_11 = ((eta_sel rR8 m, eta_sel rR9 m), (eta_sel rR10 m, eta_sel rR11 m)) in
+  let m12_15 = ((eta_sel rR12 m, eta_sel rR13 m), (eta_sel rR14 m, eta_sel rR15 m)) in
   ((m0_3, m4_7), (m8_11, m12_15))
 
 let to_fun (m:t) : (FStar.FunctionalExtensionality.restricted_t reg (fun _ -> nat64)) =
